\begin{example}
    Let
    $$
        \mat{A} = \left[\begin{matrix}
        1 & 2 & 3 \\
        4 & 5 & 6
        \end{matrix}\right],\ 
        \mat{B} = \left[\begin{matrix}
        7 & 8 & 9 \\
        1 & 2 & 3
        \end{matrix}\right]
    $$
    Then we have
    $$
        \mat{A} + \mat{B} = 
        \left[\begin{matrix}
        1+7 & 2+8 & 3+9 \\
        4+1 & 5+2 & 6+3
        \end{matrix}\right] =
        \left[\begin{matrix}
        8 & 10 & 12 \\
        5 & 7 & 9
        \end{matrix}\right]
    $$
    $$
        \transp{B} =
        \left[\begin{matrix}
        7 & 1 \\
        8 & 2 \\
        9 & 3
        \end{matrix}\right]
    $$
    $$
        \mat{A}\transp{B} =
        \left[\begin{matrix}
        1 & 2 & 3 \\
        4 & 5 & 6
        \end{matrix}\right]
        \left[\begin{matrix}
        7 & 1 \\
        8 & 2 \\
        9 & 3
        \end{matrix}\right] =
    $$
    $$
        = \left[\begin{matrix}
        1 \cdot 7 + 2 \cdot 8 + 3 \cdot 9 & 1 \cdot 1 + 2 \cdot 2 + 3 \cdot 3 \\
        4 \cdot 7 + 5 \cdot 8 + 6 \cdot 9 & 4 \cdot 1 + 5 \cdot 2 + 6 \cdot 3
        \end{matrix}\right] = 
        \left[\begin{matrix}
        50 & 14 \\
        122 & 32
        \end{matrix}\right]
    $$
\end{example}